Add sample code for conversions

Sequences/NatSeqConversions.dfy
@@ -1,12 +1,8 @@
-// TODO: Add examples of how these modules are used with assert statements
-// TODO: Add instantiation with common bounds - 8, 16, 32
-
 include "../Nonlinear_Arithmetic/DivMod.dfy"
 include "../Nonlinear_Arithmetic/Mul.dfy"
 include "../Nonlinear_Arithmetic/Power.dfy"
 include "Seq.dfy"
 include "NatSeq.dfy"
-
 
 abstract module SmallSeq refines NatSeq {
 
@@ -43,19 +39,20 @@ abstract module LargeSeq refines NatSeq {
 abstract module NatSeqConversions {
 
   import opened DivMod
-  import opened Large : LargeSeq
   import opened Mul
   import opened Power
   import opened Seq
 
+  import opened Large : LargeSeq
+
   /* Small.BOUND() to the power of E() is Large.BOUND(). */
   function method E(): nat
-    ensures power(Small.BOUND(), E()) == BOUND()
+    ensures power(Small.BOUND(), E()) == Large.BOUND()
   {
     lemma_div_basics_auto();
     lemma_power_multiplies_auto();
-    lemma_fundamental_div_mod(BITS(), Small.BITS());
-    BITS() / Small.BITS()
+    lemma_fundamental_div_mod(Large.BITS(), Small.BITS());
+    Large.BITS() / Small.BITS()
   }
 
   /* If x % y is zero and x is greater than zero, x is greater than y. */
@@ -73,7 +70,7 @@ abstract module NatSeqConversions {
   }
 
   /* Converts a sequence from Large.BOUND() to Small.BOUND(). */
-  function method {:opaque} to_small(xs: seq<uint>): (ys: seq<Small.uint>)
+  function method {:opaque} to_small(xs: seq<Large.uint>): (ys: seq<Small.uint>)
     ensures |ys| == |xs| * E()
   {
     if |xs| == 0 then []
@@ -83,7 +80,7 @@ abstract module NatSeqConversions {
   }
 
   /* Converts a sequence from Small.BOUND() to Large.BOUND(). */
-  function method {:opaque} to_large(xs: seq<Small.uint>): (ys: seq<uint>)
+  function method {:opaque} to_large(xs: seq<Small.uint>): (ys: seq<Large.uint>)
     requires |xs| % E() == 0
     ensures |ys| == |xs| / E()
   {
@@ -95,16 +92,16 @@ abstract module NatSeqConversions {
       Small.lemma_seq_nat_bound(xs[..E()]);
       lemma_mod_sub_multiples_vanish_auto();
       lemma_div_minus_one(|xs|, E());
-      [Small.to_nat(xs[..E()]) as uint] + to_large(xs[E()..])
+      [Small.to_nat(xs[..E()]) as Large.uint] + to_large(xs[E()..])
   }
 
   /* Sequence conversion from Large.BOUND() to Small.BOUND() does not
   change its nat representation. */
-  lemma lemma_to_small(xs: seq<uint>)
-    ensures Small.to_nat(to_small(xs)) == to_nat(xs)
+  lemma lemma_to_small(xs: seq<Large.uint>)
+    ensures Small.to_nat(to_small(xs)) == Large.to_nat(xs)
   {
-    reveal to_nat();
     reveal Small.to_nat();
+    reveal Large.to_nat();
     reveal to_small();
     if |xs| > 0 {
       calc {
@@ -114,9 +111,9 @@ abstract module NatSeqConversions {
             Small.lemma_seq_prefix(Small.from_nat_with_len(first(xs), E()) + to_small(drop_first(xs)), E());
             lemma_to_small(drop_first(xs));
           }
-        first(xs) + to_nat(drop_first(xs)) * power(Small.BOUND(), E());
-          { assert power(Small.BOUND(), E()) == BOUND(); }
-        to_nat(xs);
+        first(xs) + Large.to_nat(drop_first(xs)) * power(Small.BOUND(), E());
+          { assert power(Small.BOUND(), E()) == Large.BOUND(); }
+        Large.to_nat(xs);
       }
     }
   }
@@ -125,20 +122,20 @@ abstract module NatSeqConversions {
   change its nat representation. */
   lemma lemma_to_large(xs: seq<Small.uint>)
     requires |xs| % E() == 0
-    ensures to_nat(to_large(xs)) == Small.to_nat(xs)
+    ensures Large.to_nat(to_large(xs)) == Small.to_nat(xs)
   {
-    reveal to_nat();
+    reveal Large.to_nat();
     reveal Small.to_nat();
     reveal to_large();
     if |xs| > 0 {
       calc {
-        to_nat(to_large(xs));
+        Large.to_nat(to_large(xs));
           {
             lemma_mod_eq_zero(|xs|, E());
             lemma_mod_sub_multiples_vanish_auto();
             Small.lemma_seq_nat_bound(xs[..E()]);
           }
-        to_nat([Small.to_nat(xs[..E()]) as uint] + to_large(xs[E()..]));
+        Large.to_nat([Small.to_nat(xs[..E()]) as Large.uint] + to_large(xs[E()..]));
           { lemma_to_large(xs[E()..]); }
         Small.to_nat(xs[..E()]) + Small.to_nat(xs[E()..]) * power(Small.BOUND(), E());
           { Small.lemma_seq_prefix(xs, E()); }
@@ -148,15 +145,15 @@ abstract module NatSeqConversions {
   }
 
   /* to_small is injective. */
-  lemma lemma_to_small_is_injective(xs: seq<uint>, ys: seq<uint>)
+  lemma lemma_to_small_is_injective(xs: seq<Large.uint>, ys: seq<Large.uint>)
     requires to_small(xs) == to_small(ys)
     requires |xs| == |ys|
     ensures xs == ys
   {
     lemma_to_small(xs);
     lemma_to_small(ys);
-    assert to_nat(xs) == to_nat(ys);
-    lemma_seq_eq(xs, ys);
+    assert Large.to_nat(xs) == Large.to_nat(ys);
+    Large.lemma_seq_eq(xs, ys);
   }
 
   /* to_large is injective. */
@@ -188,7 +185,7 @@ abstract module NatSeqConversions {
             Small.lemma_seq_nat_bound(xs[..E()]);
             lemma_mod_sub_multiples_vanish_auto();
           }
-        to_small([Small.to_nat(xs[..E()]) as uint] + to_large(xs[E()..]));
+        to_small([Small.to_nat(xs[..E()]) as Large.uint] + to_large(xs[E()..]));
         Small.from_nat_with_len(Small.to_nat(xs[..E()]), E()) + to_small(to_large(xs[E()..]));
           {
             Small.lemma_seq_nat_seq(xs[..E()]);
@@ -201,7 +198,7 @@ abstract module NatSeqConversions {
 
   /* If we start with a Large sequence, convert it to a Sequence sequence,
   and convert it back, we get the same sequence we started with. */
-  lemma lemma_large_small_large(xs: seq<uint>)
+  lemma lemma_large_small_large(xs: seq<Large.uint>)
     ensures |to_small(xs)| % E() == 0
     ensures to_large(to_small(xs)) == xs
   {
@@ -212,7 +209,7 @@ abstract module NatSeqConversions {
       calc {
         to_large(to_small(xs));
         to_large(Small.from_nat_with_len(first(xs), E()) + to_small(drop_first(xs)));
-        [Small.to_nat(Small.from_nat_with_len(first(xs), E())) as uint] + to_large(to_small(drop_first(xs)));
+        [Small.to_nat(Small.from_nat_with_len(first(xs), E())) as Large.uint] + to_large(to_small(drop_first(xs)));
         [first(xs)] + to_large(to_small(drop_first(xs)));
           { lemma_large_small_large(drop_first(xs)); }
         [first(xs)] + drop_first(xs);
@@ -220,6 +217,22 @@ abstract module NatSeqConversions {
       }
     }
   }
+
+}
+
+module uint8_16 refines NatSeqConversions {
+
+  module uint8Seq refines SmallSeq {
+    function method BITS(): nat { 8 }
+  }
+
+  module uint16Seq refines LargeSeq {
+    import Small = uint8Seq
+    function method BITS(): nat { 16 }
+  }
+
+  import opened Large = uint16Seq
+  import Small = Large.Small
 
 }
 
@@ -235,5 +248,22 @@ module uint8_32 refines NatSeqConversions {
   }
 
   import opened Large = uint32Seq
+  import Small = Large.Small
+
+}
+
+module uint16_32 refines NatSeqConversions {
+
+  module uint16Seq refines SmallSeq {
+    function method BITS(): nat { 16 }
+  }
+
+  module uint32Seq refines LargeSeq {
+    import Small = uint16Seq
+    function method BITS(): nat { 32 }
+  }
+
+  import opened Large = uint32Seq
+  import Small = Large.Small
 
 }
