Sequences/NatSeqExample.dfy
@@ -1,0 +1,47 @@
+include "NatSeq.dfy"
+include "NatSeqConversions.dfy"
+
+include "../Nonlinear_Arithmetic/DivMod.dfy"
+include "../Nonlinear_Arithmetic/Power.dfy"
+
+module uint8_32Example {
+
+  import opened uint8_32
+
+  import opened DivMod
+  import opened Power
+
+  method Main() {
+    var n := 49602234234;
+
+    // Convert n to uint8 and uint32 sequences
+    var smallSeq, largeSeq := Small.from_nat(n), Large.from_nat(n);
+
+    Small.lemma_nat_seq_nat(n);
+    Large.lemma_nat_seq_nat(n);
+    assert Small.to_nat(smallSeq) == Large.to_nat(largeSeq) == n;
+
+    // Extend smallSeq
+    var smallExtendedLen := |smallSeq| + E() - (|smallSeq| % E());
+    lemma_sub_mod_noop_right(|smallSeq| + E(), |smallSeq|, E());
+    lemma_mod_basics_auto();
+    assert smallExtendedLen % E() == 0;
+
+    Small.lemma_seq_nat_bound(smallSeq);
+    lemma_power_increases_auto();
+    var smallSeqExtended := Small.seq_extend(smallSeq, smallExtendedLen);
+    assert Small.to_nat(smallSeqExtended) == n;
+
+    // Conversions between smallSeqExtended and largeSeq
+    lemma_to_small(largeSeq);
+    lemma_to_large(smallSeqExtended);
+    assert Small.to_nat(to_small(largeSeq)) == n;
+    assert Large.to_nat(to_large(smallSeqExtended)) == n;
+
+    lemma_small_large_small(smallSeqExtended);
+    lemma_large_small_large(largeSeq);
+    assert to_small(to_large(smallSeqExtended)) == smallSeqExtended;
+    assert to_large(to_small(largeSeq)) == largeSeq;
+  }
+
+}
